Adds itree_branch combinator and thms

pancake/semantics/proofs/panItreeSemEquivScript.sml
@@ -15,8 +15,6 @@ local open alignmentTheory
 
 val _ = new_theory "panItreeSemEquiv";
 
-Overload "case" = “itree_CASE”;
-
 Definition query_oracle_def[nocompute]:
   query_oracle ffis (FFI_call s conf bytes) = call_FFI ffis s conf bytes
 End
@@ -26,24 +24,158 @@ Definition make_io_event_def[nocompute]:
                 IO_event s conf (ZIP (bytes,rbytes))
 End
 
-(* Performs oracle trace selection and folds trace into
- result of computation, or NONE if divergent. *)
-Definition itree_oracle_outcome_def:
-  itree_oracle_outcome or t =
-  LHD $ LFLATTEN $ LUNFOLD
-           (λs. case s of
-                  SOME (or,t) =>
-                    itree_CASE t
-                               (λr. SOME (NONE,[|r|]))
-                               (λu. SOME (SOME (or,u),LNIL))
-                               (λe k. case query_oracle or e of
-                                        FFI_return or' bytes =>
-                                          SOME (SOME (or',k (FFI_return or' bytes)),LNIL)
-                                      | FFI_final (Final_event s conf bytes outcome) =>
-                                          SOME (SOME (or,k (FFI_final (Final_event s conf bytes outcome))),LNIL))
-                | NONE => NONE)
-           (SOME (or,t))
+(* Maps an itree t into a llist repr of the complete branch
+ determined by a branching choice function f. *)
+Definition itree_branch_def:
+  itree_branch f s t =
+  LUNFOLD
+  (λseed. case seed of
+         NONE => NONE
+       | SOME (t',s') =>
+           (case t' of
+              Ret r => SOME (NONE,[|r|])
+            | Tau t'' => SOME (SOME (t'',s'),LNIL)
+            | Vis e k =>
+                let (a,s'') = (f s' e) in
+                    SOME (SOME (k a,s''),LNIL)))
+  (SOME (t,s))
 End
+
+val k = “k:α -> (δ,γ,α) itree”;
+
+Theorem branch_simps[simp]:
+  (itree_branch f s (Ret r) = [|[|r|]|]) ∧
+  (itree_branch f s (Tau t) = LNIL:::(itree_branch f s t))
+Proof
+  conj_tac >>
+  rw [itree_branch_def] >>
+  rpt (rw [Once LUNFOLD])
+QED
+
+Theorem branch_bind_thm:
+  itree_branch f s (itree_bind t k) =
+  (itree_branch f s t):::(itree_branch f s (k $ THE $ LHD $ LFLATTEN $ itree_branch f s t))
+Proof
+  rw [Once LLIST_BISIMULATION] >>
+  cheat
+QED
+
+(*
+ We use itree branch to get a nice llist repr of a branch in a tree determined by f.
+ If such a branch is finite then itree_leaf will return its last element.
+*)
+
+(* Returns the result in the leaf reached by walking a semtree using the
+ specified oracle to make branching choices; or NONE for divergent trees. *)
+
+(* Do we need a concrete value or can we talk about "the value if it's ever reached"? *)
+
+(* Takes a function f : e -> a # f and an itree t, and returns either NONE for
+infinite depth paths or SOME r where r is the result in the leaf of the tree
+found by allowing f to decide branching *)
+
+Definition itree_leaf_def:
+  itree_leaf f s t = LHD $ LFLATTEN $ itree_branch f s t
+End
+
+Theorem leaf_bind_trans:
+  (k (THE (itree_leaf f s t))) = t' ⇒
+  itree_leaf f s (itree_bind t k) = itree_leaf f s t'
+Proof
+  cheat
+QED
+
+Triviality leaf_branch_thm:
+  itree_leaf f s t = SOME r ⇒
+  LHD $ LFLATTEN $ itree_branch f s t = SOME r
+Proof
+  rw [itree_leaf_def]
+QED
+
+Triviality branch_leaves_eq:
+  itree_branch f s t = itree_branch f s t' ⇒
+  itree_leaf f s t = itree_leaf f s t'
+Proof
+  rw [itree_leaf_def]
+QED
+
+
+Theorem leaf_bind_thm:
+  itree_leaf f s t = SOME r ⇒
+  itree_leaf f s (itree_bind t ^k) = itree_leaf f s (itree_bind (Ret r) k)
+Proof
+  disch_tac >>
+  rw [itreeTauTheory.itree_bind_thm] >>
+  irule branch_leaves_eq >>
+  ‘r = THE $ LHD $ LFLATTEN $ itree_branch f s t’ by (gs [itree_leaf_def]) >>
+  Cases_on ‘k r’
+  >- (rw [] >> rw [branch_bind_thm])
+QED
+
+(* Definition itree_leaf_def: *)
+(*   itree_leaf or (t:(α,β) semtree) = *)
+(*   LHD $ LFLATTEN $ LUNFOLD *)
+(*            (λs. case s of *)
+(*                   SOME (or,t) => *)
+(*                     itree_CASE t *)
+(*                                (λr. SOME (NONE,[|r|])) *)
+(*                                (λu. SOME (SOME (or,u),LNIL)) *)
+(*                                (λe k. case query_oracle or e of *)
+(*                                         FFI_return or' bytes => *)
+(*                                           SOME (SOME (or',k (FFI_return or' bytes)),LNIL) *)
+(*                                       | FFI_final (Final_event s conf bytes outcome) => *)
+(*                                           SOME (SOME (or,k (FFI_final (Final_event s conf bytes outcome))),LNIL)) *)
+(*                 | NONE => NONE) *)
+(*            (SOME (or,t)) *)
+(* End *)
+
+(* Can we prove something like:
+  - if we know the leaf of some mtree t1 and we know the leaf of some mtree t2,
+  then we know the leaf of their composition (bind) ? *)
+
+(* This would give us compositional reasoning about mtree production in the
+itree semantics. *)
+
+(* What in fact is the direct composition of trees?
+
+ - This is not what itree_bind does as it applies a tree to a function which
+produces one of a potentially infinite number of trees. *)
+
+Theorem itree_evaluate_seq_cases:
+  itree_evaluate (Seq c1 c2) s =
+  sem_outer
+  do
+    (r,s') <- itree_mrec_sem (c1,s);
+    if r = NONE then itree_mrec_sem (c2,s') else Ret (r,s')
+  od
+Proof
+  cheat
+QED
+
+(* from h_prog_rule_seq we can show that seq composition of two trees in the semantics
+ is the same as a bind with the first evaluate and an if condition that extends the tree
+    with the second evaluate so long as the first evaluate has a result of NONE.
+
+ hence:
+    h_prog_rule_seq gives:
+        (itree_evaluate p1 s) BIND (λ(res,s'). if res = NONE then itree_evaluate p2 s'))
+
+ we then need to show that itree_leaf produces the intuitive results in a bound tree:
+
+    itree_leaf (t1 BIND k) = itree_leaf
+
+
+ *)
+
+
+(* this requires a connection between itree_leaf and itree_bind *)
+(* Theorem itree_leaf_seq1: *)
+(*   itree_leaf or (itree_evaluate c1 s) = SOME (SOME r) ⇒ *)
+(*   itree_leaf or (itree_evaluate (Seq c1 c2) s) = SOME (SOME r) *)
+(* Proof *)
+(*   disch_tac >> *)
+(*     rw [itree_e] *)
+(* QED *)
 
 CoInductive itree_oracle_term_path:
   (∀x. itree_oracle_term_path or (Ret x)) ∧
@@ -75,9 +207,9 @@ Definition same_behaviour_def:
      (itree_oracle_beh or t) = ioll) ∧
   (same_behaviour or t (Terminate outcome iol) ⇔
      (∃iotrace. LTAKE (LENGTH iol) (itree_oracle_beh or t) = SOME iotrace ∧ iotrace = iol) ∧
-     (∃r. outcome = Success ⇔ (itree_oracle_outcome or t) = SOME (SOME (Return r))) ∧
-     (∃e. outcome = (FFI_outcome e) ⇔ (itree_oracle_outcome or t) = SOME (SOME (FinalFFI e)))) ∧
-  (same_behaviour or t Fail ⇔ ∃r. (itree_oracle_outcome or t) = SOME r ∧
+     (∃r. outcome = Success ⇔ (itree_leaf or t) = SOME (SOME (Return r))) ∧
+     (∃e. outcome = (FFI_outcome e) ⇔ (itree_leaf or t) = SOME (SOME (FinalFFI e)))) ∧
+  (same_behaviour or t Fail ⇔ ∃r. (itree_leaf or t) = SOME r ∧
                                   ∀e res. r ≠ SOME (FinalFFI e) ∧ r ≠ SOME (Return res))
 End
 
@@ -86,7 +218,7 @@ End
  outcomes. *)
 Definition same_outcome_def:
   same_outcome or t (SOME r,s) ⇔
-     THE (itree_oracle_outcome or t) = (SOME r)
+     THE (itree_leaf or t) = (SOME r)
 End
 
 (* Theorem same_outcome_bind_ret: *)
@@ -137,6 +269,25 @@ Proof
   cheat
 QED
 
+(* Need to be able to say:
+
+ If an itree_evaluate has some leaf BLAH, then mrec applied to some Vis will have the __same leaf__ as
+ Ret BLAH bound to the ktree from the Vis...
+
+
+ If the leaf of some tree is BLAH then the result passed to the ktree in an itree_bind is BLAH'
+
+ ----
+
+ Need also to be able to express each mrec rule involving Vis as the direct bind
+ between a tree and the corresponding ktree rather than mrec applied to a Vis node.
+
+ *)
+
+
+(* same_outcome should probably be called "itree_result" or similar *)
+
+(* Need to reason compositionally about the leaves in an itree using an oracle *)
 
 (* Need to relate same_outcome to h_prog rules
  possibly using some useful itree theorems; about binding, etc. *)
@@ -144,7 +295,11 @@ Theorem same_outcome_seq1:
   same_outcome (ffis:(β ffi_state)) (itree_evaluate (c1:(α panLang$prog)) s) (SOME r,s':((α,β) state)) ⇒
   same_outcome ffis (itree_evaluate (Seq c1 c2) s) (SOME r,s')
 Proof
-  cheat
+  disch_tac >>
+  rw [panItreeSemTheory.itree_evaluate_def] >>
+  rw [panItreeSemTheory.itree_mrec_def] >>
+  rw [panItreeSemTheory.h_prog_def] >>
+  rw [panItreeSemTheory.h_prog_rule_seq_def] >>
 QED
 
 Theorem same_outcome_seq2:
@@ -188,7 +343,7 @@ Proof
       rw [itreeTauTheory.itree_iter_def] >>
       rw [Once itreeTauTheory.itree_unfold] >>
       rw [Once itreeTauTheory.itree_unfold] >>
-      rw [itree_oracle_outcome_def] >>
+      rw [itree_leaf_def] >>
       rw [Once LUNFOLD]
       (* Case: everything evaluates as expected *)
       >- (rw [query_oracle_def] >>
@@ -257,7 +412,7 @@ Proof sketch:
       rw [Once itreeTauTheory.itree_unfold] >>
       rw [Once itreeTauTheory.itree_unfold] >>
       rw [same_outcome_def] >>
-      rw [itree_oracle_outcome_def] >>
+      rw [itree_leaf_def] >>
       rw [Once LUNFOLD] >>
       rw [itreeTauTheory.itree_bind_def]
       (* Case: evaluating the callee returns (NONE,s') *)
@@ -280,7 +435,7 @@ Proof sketch:
           ‘eval (s with <|clock := k; ffi := ffis|>) e = NONE’ by rw [GSYM fbs_eval_clock_and_ffi_eq] >>
           fs[] >>
           rw [Once itreeTauTheory.itree_unfold] >>
-          rw [itree_oracle_outcome_def] >>
+          rw [itree_leaf_def] >>
           rw [Once LUNFOLD])
       (* eval s e = SOME x *)
       >- (
@@ -288,62 +443,6 @@ Proof sketch:
        )
       )
 QED
-
-(* Useful garbage *)
-(* fs [CaseEqs ["option"]] *)
-(* >- (rw [panItreeSemTheory.itree_evaluate_def] >> *)
-(*     rw [panItreeSemTheory.itree_mrec_def] >> *)
-(*     rw [panItreeSemTheory.h_prog_def] >> *)
-(*     rw [panItreeSemTheory.h_prog_rule_ext_call_def] >> *)
-(*     ‘eval s ptr1 = eval (s with <|clock := k; ffi := ffis|>) ptr1’ by rw [fbs_eval_clock_and_ffi_eq] >> *)
-(*     fs [] >> *)
-(*     rw [Once itreeTauTheory.itree_unfold] >> *)
-(*     rw [same_outcome_def] >> *)
-(*     rw [itree_oracle_outcome_def] >> *)
-(*     rw [Once LUNFOLD] *)
-(*    ) *)
-(* >- (full_case_tac >> *)
-(*     rw [panItreeSemTheory.itree_evaluate_def] >> *)
-(*     rw [panItreeSemTheory.itree_mrec_def] >> *)
-(*     rw [panItreeSemTheory.h_prog_def] >> *)
-(*     rw [panItreeSemTheory.h_prog_rule_ext_call_def] >> *)
-(*     ‘eval s len2 = eval (s with <|clock := k; ffi := ffis|>) len2’ by rw [fbs_eval_clock_and_ffi_eq] >> *)
-(*     ‘eval s ptr1 = eval (s with <|clock := k; ffi := ffis|>) ptr1’ by rw [fbs_eval_clock_and_ffi_eq] >> *)
-(*     fs [] >> *)
-(*     (* STILL NEED TO REDUCE CASE EXPR *) *)
-(*   ) *)
-(* Elim all these cases as at least one eval is NONE *)
-(* rw [panItreeSemTheory.itree_evaluate_def] >> *)
-(* rw [same_outcome_def] >> *)
-(* rw [itree_oracle_outcome_def] >> *)
-(* rw [panItreeSemTheory.itree_mrec_def] >> *)
-(* rw [panItreeSemTheory.h_prog_def] >> *)
-(* rw [panItreeSemTheory.h_prog_rule_ext_call_def] >> *)
-(* ‘eval s len2 = eval (s with <|clock := k; ffi := ffis|>) len2’ by rw [fbs_eval_clock_and_ffi_eq] >> *)
-(* ASSUM_LIST (fn thl => ‘eval s len2 = NONE’ by (rw thl)) >> *)
-
-
-(* EVERY_CASE_TAC >> *)
-(* rw [Once itreeTauTheory.itree_unfold] >> *)
-(* rw [same_outcome_def] >> *)
-(* rw [itree_oracle_outcome_def] >> *)
-(* rw [Once LUNFOLD] *)
-(* How to reduce a case where every outcome is the same to that outcome? *)
-
-(* >- (EVERY_CASE_TAC >> *)
-(*     rw [panItreeSemTheory.itree_evaluate_def] >> *)
-(*     rw [panItreeSemTheory.itree_mrec_def] >> *)
-(*     rw [panItreeSemTheory.h_prog_def] >> *)
-(*     rw [panItreeSemTheory.h_prog_rule_ext_call_def] >> *)
-(*     ‘eval s ptr1 = eval (s with <|clock := k; ffi := ffis|>) ptr1’ by rw [fbs_eval_clock_and_ffi_eq] >> *)
-(*     POP_ASSUM_LIST (fn thl => ‘eval s ptr1 = NONE’ by (rw thl)) >> *)
-(*     rw [] >> *)
-(*     rw [Once itreeTauTheory.itree_unfold] >> *)
-(*     rw [same_outcome_def] >> *)
-(*     rw [itree_oracle_outcome_def] >> *)
-(*         rw [Once LUNFOLD]) *)
-(* ) *)
-
 
 (* Final goal:
 
